SuperKlon.dfy
@@ -1,13 +1,390 @@
 
-///have to sort out c_amfx -- make sure it makes sense
+//[[[[[[[[[[[[[[[[[[[[[[[[[[[[[[[[[[[[[[[[]]]]]]]]]]]]]]]]]]]]]]]]]]]]]]]]]]]]]]]]
+//[[[[[[[[[[[[[[[[[[[[[[[[[[[[[[[[[[[[[[[[]]]]]]]]]]]]]]]]]]]]]]]]]]]]]]]]]]]]]]]]
 
-function {:axiom} FAKE() : Object
 
-type SuperKlon = m : Klon | wexford2(m)
-  witness Klon(map[],
-               FAKE(),
-               {}, {}, {}, {}, {})
-//not sure about this. but...
+function  OOOLDEklonKV(c' : Klon, k : Object, v : Object) : (m : Klon)
+  requires k !in c'.m.Keys
+  requires v !in c'.m.Values
+  requires klonCanKV(c', k, v)
+
+reads k`fields, k`fieldModes
+reads v`fields, v`fieldModes
+reads c'.oHeap`fields, c'.oHeap`fieldModes
+reads c'.ns`fields, c'.ns`fieldModes
+// reads c'.o`fields, c'.o`fieldModes
+
+reads c'.m.Values`fieldModes
+reads c'.m.Keys`fieldModes
+
+
+
+{
+  klonKV(c', k, v)
+}
+
+function OOOLDEmapThruKlon(os: set<Object>, m : Klon) : (r : set<Object>)
+  //image of os under klon mapping m
+  // reads m.m.Keys`fields, m.m.Keys`fieldModes
+  // reads m.m.Values`fields, m.m.Values`fieldModes
+  requires os <= m.m.Keys
+{ set o <- os :: m.m[o] }
+
+
+//[[[[[[[[[[[[[[[[[[[[[[[[[[[[[[[[[[[[[[[[]]]]]]]]]]]]]]]]]]]]]]]]]]]]]]]]]]]]]]]]
+//[[[[[[[[[[[[[[[[[[[[[[[[[[[[[[[[[[[[[[[[]]]]]]]]]]]]]]]]]]]]]]]]]]]]]]]]]]]]]]]]
+//somwhere need series of "states"  pr "steps" pr "lemmata" of the Klon state
+//1. created
+//2. all owners of o in m.Keys  (Klown)
+//3. ??>
+//4. all owners & all fields of o in m.Keys ==> NEARLY DONE
+//5. all o (and thus owners & all fields of o) in m.Keyes ==> DONE
+//
+// key preconditions
+// all an object's owners are added before the object itself is added
+// an object is added before its fields are added:
+// ...BUT we never RETURN from a meethod that creates an object
+//  UNTIL that object is fully populatioend with FIELDS
+
+function   mapThruKlown(k : Object, m : Klon) : Owner
+  requires k in m.m.Keys
+  // requires v in m.m.Values
+  // requires m.m[k] == v
+  requires m.o_amfo <= m.m.Keys   //IN-KLON
+  requires k.owner <= m.m.Keys   //IN-KLON
+  requires k.AMFO  <= m.m.Keys   //IN-KLON
+  reads m.oHeap`fields, m.oHeap`fieldModes
+  reads m.ns`fields, m.ns`fieldModes
+{
+  mapKlown(k.AMFO, m)
+}
+
+function mapKlown(k : Owner, m : Klon) : Owner
+  requires m.o_amfo <= m.m.Keys   //KLON-OK
+  requires k <= m.m.Keys
+  reads m.oHeap`fields, m.oHeap`fieldModes
+  reads m.ns`fields, m.ns`fieldModes
+{
+  var CXTRA := m.c_amfx - mapThruKlon(m.o_amfo, m);
+  var OXTRA := mapThruKlon(m.o_amfo, m) - m.c_amfx;
+
+//  assert  (mapThruKlon(m.o_amfo, m) - OXTRA + CXTRA) == m.c_amfx;
+
+  (mapThruKlon(k,m) - OXTRA + CXTRA )
+}
+
+
+lemma LEMMAMapKlown(k : Owner, m : Klon)
+  requires m.o_amfo <= m.m.Keys   //IN-KLON
+  requires k <= m.m.Keys
+{
+  var CXTRA := m.c_amfx - mapThruKlon(m.o_amfo, m);
+  var OXTRA := mapThruKlon(m.o_amfo, m) - m.c_amfx;
+
+  assert  (mapThruKlon(m.o_amfo, m) - OXTRA + CXTRA) == m.c_amfx;
+}
+
+lemma KLUCKO(o : Object, m : Klon)
+   requires m.readyOK(o)
+   ensures  o.Ready()
+   ensures  o in m.m.Keys
+   ensures  o.owner <= m.m.Keys
+   ensures  o.AMFO  <= m.m.Keys
+{}
+
+// predicate objectOwnerAttributesMapOK(o : Object, m : Klon)
+// //nicer? version of klownMapOK?
+// //do all o's owner attribute map to m.m[o]'s attributes
+// //not currently needed?
+//   requires m.o_amfo <= m.m.Keys   //KLON-OK
+//   requires m.m.Keys >= o.ntrnl > o.owner >= o.bound  //IN-KLON
+//   requires m.m.Keys >= o.AMFO  > o.AMFX  >= o.AMFB   //IN-KLON
+//   requires o in m.m.Keys  //IN-KLON
+  // reads m.oHeap`fields, m.oHeap`fieldModes
+  // reads m.ns`fields, m.ns`fieldModes
+// {
+//   var c := m.m[o];
+//
+//   && (c.bound == mapKlown(o.bound, m))
+//   && (c.AMFB  == mapKlown(o.AMFB,  m))
+//   && (c.owner == mapKlown(o.owner, m))
+//   && (c.AMFX  == mapKlown(o.AMFX , m))
+//   && (c.ntrnl == mapKlown(o.ntrnl, m))
+//   && (c.AMFO  == mapKlown(o.AMFO,  m))  ///KJX HUMM
+// }
+
+
+
+predicate {:isolate_assertions} klownMapOK(o : Object, m : Klon)
+//do all o's owner attributes map through m?
+//kjx: don't really need that v parameter do we?
+//kjx: see allklownMapOK for why k & v must be in m already
+
+  // requires m.o_amfo <= m.m.Keys   //KLON-OK
+  // requires m.m.Keys >= o.ntrnl > o.owner >= o.bound  //IN-KLON
+  // requires m.m.Keys >= o.AMFO  > o.AMFX  >= o.AMFB   //IN-KLON
+  // requires o in m.m.Keys  //IN-KLON
+
+  requires m.o_amfo <= m.m.Keys   //KLON-OK
+  requires m.readyOK(o)
+  requires (KLUCKO(o,m); o.Ready())//BUGGY!
+  requires o.Ready()
+  requires m.m.Keys >= o.bound
+  requires m.m.Keys >= o.ntrnl > o.owner >= o.bound  //IN-KLON
+  requires m.m.Keys >= o.AMFO  > o.AMFX  >= o.AMFB   //IN-KLON
+  requires o.owner <= m.m.Keys   //IN-KLON
+  requires o.AMFO  <= m.m.Keys   //IN-KLON
+
+  reads m.oHeap`fields, m.oHeap`fieldModes
+  reads m.ns`fields, m.ns`fieldModes
+  reads m.m.Keys`fields, m.m.Keys`fieldModes
+{
+  var c := m.m[o];
+
+  && (c.bound == mapKlown(o.bound, m))
+  && (c.AMFB  == mapKlown(o.AMFB,  m))
+  && (c.owner == mapKlown(o.owner, m))
+  && (c.AMFX  == mapKlown(o.AMFX , m))
+  && (c.ntrnl == mapKlown(o.ntrnl, m))
+  && (c.AMFO  == mapKlown(o.AMFO,  m))
+}
+
+
+
+
+lemma  MapKlownMapsOK1(k : Object, v : Object, m : Klon)
+  requires m.o_amfo <= m.m.Keys   //KLON-OK
+  requires m.readyOK(k)
+  requires k in m.m.Keys
+  requires k.Ready()
+  requires m.m.Keys >= k.ntrnl > k.owner >= k.bound  //IN-KLON
+  requires m.m.Keys >= k.AMFO  > k.AMFX  >= k.AMFB   //IN-KLON
+  requires k.owner <= m.m.Keys   //IN-KLON
+  requires k.AMFO  <= m.m.Keys   //IN-KLON
+
+  requires m.readyOK(k)
+  requires k in m.m.Keys
+  requires v in m.m.Values
+  requires m.m[k] == v
+  requires m.o_amfo <= m.m.Keys   //IN-KLON
+  requires k.owner <= m.m.Keys   //IN-KLON
+  requires k.AMFO  <= m.m.Keys   //IN-KLON
+  requires klownMapOK(k,m)
+  ensures (
+    var mTKoA := mapThruKlon(m.o_amfo, m);
+    var CXTRA := m.c_amfx - mTKoA;
+    var OXTRA := mTKoA - m.c_amfx;
+    && ((mTKoA - OXTRA + CXTRA) == m.c_amfx)
+    && (v.AMFO == mapThruKlown(k,m))
+  )
+{
+    var mTKoA := mapThruKlon(m.o_amfo, m);
+    var CXTRA := m.c_amfx - mTKoA;
+    var OXTRA := mTKoA - m.c_amfx;
+    assert
+      && ((mTKoA - OXTRA + CXTRA) == m.c_amfx)
+      && (v.AMFO == mapThruKlown(k,m))
+      ;
+}
+
+
+
+predicate {:isolate_assertions} allklownMapOK(m : Klon) : (rv : bool)
+//   requires forall k <- m.m.Keys :: k.owner <= m.m.Keys   //IN-KLON
+//   requires forall k <- m.m.Keys :: k.AMFO  <= m.m.Keys   //IN-KLON
+//
+//
+  requires m.readyAll()
+  requires m.o_amfo <= m.m.Keys //KLON-OK
+  //requires forall k <- m.m.Keys :: m.readyOK(k)
+
+  reads m.oHeap`fields, m.oHeap`fieldModes
+  reads m.ns`fields, m.ns`fieldModes
+  reads m.m.Keys`fields, m.m.Keys`fieldModes
+//  ensures  rv ==> (forall x <- m.m.Keys :: klownMapOK(x,m))
+{
+  forall x <- m.m.Keys ::
+    (
+    // && x in m.m.Keys
+    && m.readyOK(x)
+    && (KLUCKO(x,m); x.Ready())//BUGGY!
+    // && x.owner <= m.m.Keys
+    // && x.AMFO  <= m.m.Keys
+    && klownMapOK(x,m)
+   )
+}
+
+lemma AllKlownMapKVRestored(m' : Klon, k : Object, v : Object, m : Klon)
+//Horrible name, but OKs adding a new cloned object into the klon.
+//ensures m'[k := v] == m
+  requires k !in m'.m.Keys
+  requires v !in m'.m.Values
+  requires m'.ownersInKlown(k)
+
+  // requires forall k <- m'.m.Keys :: k.owner <= m'.m.Keys   //IN-KLON
+  // requires forall k <- m'.m.Keys :: k.AMFO  <= m'.m.Keys   //IN-KLON
+
+  requires m'.readyAll()
+  requires m'.o_amfo <= m'.m.Keys   //KLON-OK
+  requires allklownMapOK(m')
+
+  requires k.Ready()
+
+requires m.m.Keys >= k.bound
+requires m.m.Keys >= k.ntrnl > k.owner >= k.bound  //IN-KLON
+requires m.m.Keys >= k.AMFO  > k.AMFX  >= k.AMFB   //IN-KLON
+requires k.owner <= m.m.Keys   //IN-KLON
+requires k.AMFO  <= m.m.Keys   //IN-KLON
+
+
+  //preconds or allklownMapOK(m)
+  requires m == klonKV(m',k,v)
+  requires k.owner <= m.m.Keys   //IN-KLON
+  requires k.AMFO  <= m.m.Keys   //IN-KLON
+  requires klownMapOK(k,m)
+
+  ensures  allklownMapOK(m)
+
+
+{
+//   assert v == m.m[k];
+//   assert forall mm <- m'.m.Keys :: m'.m[mm]  == m.m[mm];
+//   assert forall mm <- m.m.Keys :: ((mm in m'.m.Keys) ==> (m'.m[mm] == m.m[mm]));
+//
+//   assert m.m.Keys == m'.m.Keys + {k};
+//
+//    assert allklownMapOK(m');
+//    assert forall mm <- m'.m.Keys       :: klownMapOK(mm, m);
+//    assert klownMapOK(k,m);
+//    assert forall mm <- {k}             :: klownMapOK(mm, m);
+//    assert forall mm <- m'.m.Keys + {k} :: klownMapOK(mm, m);
+//    assert forall mm <- m.m.Keys        :: klownMapOK(mm, m);
+//    assert allklownMapOK(m);
+}
+
+
+lemma {:isolate_assertions} AllKlownPreservesOwnership(m : Klon)
+
+  //preconds or allklownMapOK(m)
+  requires m.readyAll()
+  requires m.o_amfo <= m.m.Keys //KLON-OK
+
+  requires allklownMapOK(m)
+  requires forall k <- m.m.Keys :: k.owner <= m.m.Keys   //IN-KLON
+  requires forall k <- m.m.Keys :: k.AMFO  <= m.m.Keys   //IN-KLON
+  requires m.o_amfo <= m.m.Keys//KLON-OK
+
+
+  ensures forall i <- m.m.Keys, j <- m.m.Keys ::  (insideCompatible(i,j,m.m[i],m.m[j],m))
+
+  {
+assert forall i <- m.m.Keys :: klownMapOK(i,m);
+
+forall i <- m.m.Keys, j <- m.m.Keys
+  ensures (insideCompatible(i,j,m.m[i],m.m[j],m))
+  {
+    if (i == j) { return; }
+    if (inside(i,j)) {
+        assert i.AMFO >= j.AMFO;
+        assert klownMapOK(i,m);
+        assert klownMapOK(j,m);
+    }
+    assert (insideCompatible(i,j,m.m[i],m.m[j],m));
+  }
+
+//  assert forall i <- m.m.Keys, j <- m.m.Keys ::  (insideCompatible(i,j,m.m[i],m.m[j],m));
+
+  }
+
+
+
+lemma {:isolate_assertions} AllKlownPreservesReferences(m : Klon)
+
+  //preconds or allklownMapOK(m)
+  requires m.readyAll()
+  requires m.o_amfo <= m.m.Keys //KLON-OK
+
+  requires allklownMapOK(m)
+  requires forall k <- m.m.Keys :: k.owner <= m.m.Keys   //IN-KLON
+  requires forall k <- m.m.Keys :: k.AMFO  <= m.m.Keys   //IN-KLON
+  requires m.o_amfo <= m.m.Keys//KLON-OK
+
+  requires forall i <- m.m.Keys, j <- m.m.Keys ::  (insideCompatible(i,j,m.m[i],m.m[j],m))
+
+  ensures  forall i <- m.m.Keys, j <- m.m.Keys ::  (refOK(i,j) ==> refOK(m.m[i],m.m[j]))
+
+  {
+assert forall i <- m.m.Keys :: klownMapOK(i,m);
+
+
+forall i <- m.m.Keys, j <- m.m.Keys
+  ensures (refOK(i,j) ==> refOK(m.m[i],m.m[j]))
+  {
+    if refOK(i,j) {
+      if (i == j) {
+        assert refOK(m.m[i],m.m[j]);
+      } else if (refBI(i,j)) {
+          assert refBI(m.m[i],m.m[j]);
+          assert refOK(m.m[i],m.m[j]);
+      } else if (refDI(i,j)) {
+          assert refDI(m.m[i],m.m[j]);
+          assert refOK(m.m[i],m.m[j]);
+      } else {
+        assert {:contradiction} not(refOK(i,j));
+        assert {:contradiction} false;
+      }
+    }
+    assert (refOK(i,j) ==> refOK(m.m[i],m.m[j]));
+  }
+
+
+
+
+  }
+
+
+
+
+
+
+
+
+predicate insideCompatible(of : Object, ot : Object, cf : Object, ct: Object, m : Klon) : ( rv : bool )
+  //clone's inside is compatible with original's inside
+  requires {of, ot} <= m.m.Keys
+  requires m.m[of] == cf
+  requires m.m[ot] == ct
+{
+  (inside(of,ot) ==> inside(cf,ct))
+}
+
+
+
+//[[[[[[[[[[[[[[[[[[[[[[[[[[[[[[[[[[[[[[[[]]]]]]]]]]]]]]]]]]]]]]]]]]]]]]]]]]]]]]]]
+//[[[[[[[[[[[[[[[[[[[[[[[[[[[[[[[[[[[[[[[[]]]]]]]]]]]]]]]]]]]]]]]]]]]]]]]]]]]]]]]]
+// paranoid self-consistency checks
+
+
+lemma MoreValidThanValid(o : Object)
+  requires o.Ready()
+  ensures  o !in o.AMFB
+  ensures  o !in o.AMFX
+  ensures  o  in o.AMFO
+{}
+
+lemma OOOLDEInside3(a : Object, b : Object, c : Object)
+  requires inside(a,b)
+  requires inside(b,c)
+  ensures  inside(a,c)
+{}
+
+
+
+
+
+
+//diversion -BI & DI definitions cross with flattness
+//predicate fefBI(f : Object, t : Object) {flatten(f.bound) >= flatten(t.owner)}
 
 lemma recBIvsfefBI(f : Object, t : Object)
   requires f.Ready()
@@ -28,13 +405,6 @@ lemma recDIvsFLAT(f : Object, t : Object)
   ensures (f.AMFO == t.AMFX) ==> ((flatten(f.ntrnl - {f}) + {f})  == flatten(t.owner))
 {}
 
-
-lemma MoreValidThanValid(o : Object)
-  requires o.Ready()
-  ensures  o !in o.AMFB
-  ensures  o !in o.AMFX
-  ensures  o  in o.AMFO
-{}
 
 lemma refBI_nesting(a : Object, b : Object, c : Object, m : Klon)
   requires a.Ready()
@@ -61,18 +431,21 @@ lemma refBI_transitive(a : Object, b : Object, c : Object, m : Klon)
   ensures  refBI(a,c)
 {}
 
+//end diversion
+
+
 //
 // derived lemmas equality etc
 //
 
-lemma {:axiom}  AXIOMAMFOS(a : Object, b : Object)
+lemma AXIOMAMFOS(a : Object, b : Object)
 // equal AMFOs iff same objects
   requires a.Ready()
   requires b.Ready()
   ensures  (a == b)  ==> (a.AMFO == b.AMFO)
   ensures  (a == b) <==  (a.AMFO == b.AMFO)
   ensures  (a == b) <==> (a.AMFO == b.AMFO)
-
+{}
 
 
 lemma AXIOMAMFO(part : Object, whole : Object)
@@ -102,53 +475,33 @@ lemma AXIOMAMFOREVERSE(part : Object, whole : Object)
 // inside vs inside
 //
 
-lemma fuckenOwnerReady(part : Object, whole : Object)
-    requires part.Ready()
-    ensures  forall  x <- part.owner :: x.Ready()
-    ensures  forall  x <- part.owner :: part.AMFO > x.AMFO
-{}
-
 predicate recInside(part : Object, whole : Object) : (r : bool)
-    requires part.SKReady()
+    requires part.Ready()
     decreases part.AMFO
 {
-//  forall x | x in part.owner ensures (true) { fuckenOwnerReady(x, whole); }
-
   || (part == whole)
-  || (exists x <- part.owner ::
-        && (x.SKReady())                ////grr should be unnecessary
-        && (part.AMFO > x.AMFO)       ////grr should be unnecessary
-        && (recInside(x,whole)))
+  || (exists x <- part.owner :: recInside(x,whole))
 }
 
 function collectAllOwners(o : Object) : (rv : Owner)
   decreases o.AMFO
-  requires  o.Ready()
-  requires  o.OvenReady()
-  requires  o.SKReady()
+  requires o.Ready()
 {
-  o.fucked(o);
   {o} + o.owner + (set xo <- o.owner, co <- collectAllOwners(xo) :: co)
 }
 
 lemma collectAllAMFO(o : Object)
   decreases o.AMFO
   requires  o.Ready()
-  requires  o.SKReady()
   ensures   o.AMFO == collectAllOwners(o)
-  {
-      o.OvenReadyReady();
-  }
+  {}
 
-lemma {:isolate_assertions} recInsideCollectsAllOwners1(part : Object, whole : Object)
+lemma recInsideCollectsAllOwners1(part : Object, whole : Object)
   decreases part.AMFO
   requires part.Ready()
-  requires part.SKReady()
   requires recInside(part,whole)
   ensures  (whole in collectAllOwners(part))
-{
-  //  part.OvenReadyReady();
-}
+{}
 
 lemma recInsideCollectsAllOwners2(part : Object, whole : Object)
   decreases part.AMFO
@@ -156,42 +509,45 @@ lemma recInsideCollectsAllOwners2(part : Object, whole : Object)
   ensures recInside(part,whole) <== (whole in collectAllOwners(part))
 {}
 
-// lemma {:isolate_assertions} recInsideCollectsAllOwners2(part : Object, whole : Object)
-//   decreases part.AMFO
-//   requires part.SKReady()
-//   requires part.Ready()
-//   requires part.OvenReady()
-//   requires (whole in collectAllOwners(part))
-//   ensures  recInside(part,whole)
-// {
-//     part.OvenReadyReady();
-// }
+
+
+
+
+
 
 lemma recInsideAMFO1(part : Object, whole : Object)
   decreases part.AMFO
   requires part.Ready()
-  requires part.SKReady()
-////  requires whole.Ready() //why not?
+  requires whole.Ready() //why not?
 
   requires (whole in part.AMFO)
   ensures  recInside(part,whole)
-{
-      part.OvenReadyReady();
-}
+{}
 
 lemma recInsideAMFO2(part : Object, whole : Object)
   decreases part.AMFO
-  requires part.Ready()
-  requires part.SKReady()
-//  requires  whole.Ready() //why not?
+  requires  part.Ready()
+  requires  whole.Ready() //why not?
   requires  recInside(part,whole)
   ensures   (whole in part.AMFO)
 {}
 
+lemma InsideRecInside1(part : Object, whole : Object)
+   requires part.Ready()
+   requires whole.Ready() //why not?
+   requires recInside(part,whole)
+   ensures  inside(part,whole)
+   {
+      recInsideCollectsAllOwners1(part,whole);
+      assert (whole in collectAllOwners(part));
+      collectAllAMFO(part);
+      assert (whole in part.AMFO);
+      AXIOMAMFO(part, whole);
+   }
+
 
 lemma InsideRecInside2(part : Object, whole : Object)
    requires part.Ready()
-   requires part.SKReady()
    requires whole.Ready() //why not?
    requires    inside(part,whole)
    ensures  recInside(part,whole)
@@ -206,19 +562,6 @@ lemma InsideRecInside2(part : Object, whole : Object)
     assert recInside(part,whole);
    }
 
-lemma InsideRecInside1(part : Object, whole : Object)
-   requires part.Ready()
-   requires part.SKReady()
-// requires whole.Ready() //why not?
-   requires recInside(part,whole)
-   ensures  inside(part,whole)
-   {
-      recInsideCollectsAllOwners1(part,whole);
-      assert (whole in collectAllOwners(part));
-      collectAllAMFO(part);
-      assert (whole in part.AMFO);
-      AXIOMAMFO(part, whole);
-   }
 
 
 
@@ -228,12 +571,14 @@ lemma AMFOsisAMFOs(o : Object)
 {}
 
 
+
+
+
 ///////////////////////////////////////////////////////////////////////////////////////////
 // the Pointing Lemmas
 ///////////////////////////////////////////////////////////////////////////////////////////
-
-lemma
-INSIDE_CAN_POUNT_OUT(m' : Klon, f : Object, t : Object, o : Object, c : Object)
+//
+lemma INSIDE_CAN_POUNT_OUT(m' : Klon, f : Object, t : Object, o : Object, c : Object)
  requires f.Ready()
  requires o.Ready()
  requires t.Ready()
@@ -321,1912 +666,3 @@ lemma INCOMING_REFS_OWNER_ONLY(f : Object, t : Object, o : Object)
  ensures  t == o
  ensures f != t
 {}
-
-
-
-function  subklonKV(m' : Klon, k : Object, v : Object) : (m : Klon)
-  requires k !in m'.m.Keys
-  requires v !in m'.m.Values
-{
-      reveal UniqueMapEntry();
-m'.(m:=m'.m[k:=v])  //l.(m:=l.m[k:=v])
-}
-
-
-
-lemma {:verify false} KVdexy(m' : Klon, k : Object, v : Object, m : Klon)
-//the whole thing!
-//this one is on ice, cos we're choppint up the KVscartchmonkey version...
-  requires k !in m'.m.Keys
-  requires v !in m'.m.Values
-  requires m == subklonKV(m',k,v)
-
-  requires k.Ready()
-  requires v.Ready()
-  requires forall k <- m'.m.Keys :: k.Ready() && m.m[k].Ready()
-
-  requires allmagic2(m')
-
-
-  requires magic2(k,v,m')
-  ensures  allmagic2(m)
-
-  requires dexford4(m')
-  // ensures  dexford4(m)
-
-  {
-
-
-forall i <- m.m.Keys, j <- m.m.Keys
-   ensures dexy_NO_builtin(i,j,m.m[i],m.m[j],m)
-   {
-      var of := i; var ot := j;  var cf := m.m[i]; var ct := m.m[j];
-      //original from, original to, clone from, clone to
-
-
-  if ((of != k) && (ot != k)) { //already in m', so already OK
-
-    kvdNOTKK(m', k, v, of, ot, cf, ct, m);
-
-        // assert dexy_NO_builtin(i,j,m.m[i],m.m[j],m);
-        // assert (refOK(of,ot) ==> refOK(cf,ct));
-    } else {
-      //at least one of of and ot are k
-  if (of == ot) {  //both are!
-
-    kvdEQKK(m', k, v, of, ot, cf, ct, m);
-
-    } else {
-
-
-    assert of != ot;
-    assert (of == k) != (ot == k);
-    //from here on, of one of and ot is k, the other is not
-
-  if (refDI(of,ot) && (of == k)) {//refDI(k,ot)
-
-    assert ot != k;
-    assert of.AMFO == ot.AMFX;  //by defn DI
-
-  //  kdvDIKN(m', k, v, of, ot, cf, ct, m);
-
-    if (k == v) {
-      assert not(of.AMFO >= m.o_amfo); //k outside
-      assert of == cf == v == k; //k outside
-      // assert refOK(k,v);
-      // assert ct == m.m[ot];
-      // assert magic(ot,ct,m);
-
-      assert of.AMFO == ot.AMFX;  //ref defin DI
-      assert of.AMFO != m.o_amfo;
-
-      assert not(of.AMFO >= m.o_amfo);
-
-      if (ot.AMFX == m.o_amfo) { //directly inside
-          assert ((ot != ct) && (ct.AMFX == m.c_amfx));
-          assert refOK(of,ot);
-          assert refOK(cf,ct);
-        } else  {
-          assert refOK(cf,ct);
-          assert (refOK(of,ot) ==> refOK(cf,ct));
-        }
-
-      assert (refOK(of,ot) ==> refOK(cf,ct));
-
-      } else {
-        assert ((v != k) && (v.AMFO >= m.c_amfx));  //inside & cloned
-
-        assert (refOK(of,ot) ==> refOK(cf,ct));
-      }
-        assert refOK(v,ct);
-        assert wexy_NO_builtin(i,j,m.m[i],m.m[j],m);
-        } else {
-
-
-
-      if (refDI(of,k)) {
-
-
-      if (ot.AMFX == m.o_amfo) { //directly inside
-          assert ((ot != ct) && (ct.AMFX == m.c_amfx));
-          assert refOK(of,ot);
-          assert refOK(cf,ct);
-
-        assume refOK(cf,k);
-        }} else {
-      if (refBI(of,ot)) {
-        assume refOK(cf,ct);
-       } else {
-        assert not(refOK(of,ot));
-        assert dexy_NO_builtin(i,j,m.m[i],m.m[j],m);
-       }}}}}
-
-
-assume dexy_NO_builtin(i,j,m.m[i],m.m[j],m);
-
-
-   } //end of FORALL statement
-
-// var i := k;  assert (forall j <- m'.m.Keys :: wexy_NO_builtin(i,j,m.m[i],m.m[j],m));
-// var j := k;  assert (forall i <- m'.m.Keys :: wexy_NO_builtin(i,j,m.m[i],m.m[j],m));
-
-  assert (forall i <- m.m.Keys, j <- m.m.Keys :: dexy_NO_builtin(i,j,m.m[i],m.m[j],m));
-
-}//done lemma KVdexy
-
-
-
-
-
-
-
-
-
-
-
-
-
-
-
-
-
-
-
-
-
-
-
-
-
-
-
-
-
-
-
-
-
-
-
-
-lemma {:verify false} KVscratchmonkey(m' : Klon, k : Object, v : Object, m : Klon)
-//the whole thing!
-//current dev version of KVdexy...
-//aim is to go through cbopping out cases as sublemmas kvdXXX
-  requires k !in m'.m.Keys
-  requires v !in m'.m.Values
-  requires m == subklonKV(m',k,v)
-
-  requires k.Ready()
-  requires v.Ready()
-  requires forall k <- m'.m.Keys :: k.Ready() && m.m[k].Ready()
-
-  requires allmagic2(m')
-
-
-  requires magic2(k,v,m')
-//  ensures  allmagic2(m)
-
-  requires dexford4(m')
-  // ensures  dexford4(m)
-  {
-
-
-forall i <- m.m.Keys, j <- m.m.Keys
-   ensures true
-//   ensures dexy_NO_builtin(i,j,m.m[i],m.m[j],m)
-   {
-      var of := i; var ot := j;  var cf := m.m[i]; var ct := m.m[j];
-      //original from, original to, clone from, clone to
-
-
-  if ((of != k) && (ot != k)) { //already in m', so already OK
-
-    kvdNOTKK(m', k, v, of, ot, cf, ct, m);
-
-        // assert dexy_NO_builtin(i,j,m.m[i],m.m[j],m);
-        // assert (refOK(of,ot) ==> refOK(cf,ct));
-    } else {
-      //at least one of of and ot are k
-  if (of == ot) {  //both are!
-
-    kvdEQKK(m', k, v, of, ot, cf, ct, m);
-
-    } else {
-
-
-    assert of != ot;
-    assert (of == k) != (ot == k);
-    //from here on, of one of and ot is k, the other is not
-
-  if (refDI(of,ot) && (of == k)) {//refDI(k,ot)
-
-    assert ot != k;
-    assert of.AMFO == ot.AMFX;  //by defn DI
-
-//    kdvDIKN(m', k, v, of, ot, cf, ct, m);
-
-    if (k == v) {
-      assert not(of.AMFO >= m.o_amfo); //k outside
-      assert of == cf == v == k; //k outside
-      // assert refOK(k,v);
-      // assert ct == m.m[ot];
-      // assert magic(ot,ct,m);
-
-      assert of.AMFO == ot.AMFX;  //ref defin DI
-      assert of.AMFO != m.o_amfo;
-
-      assert not(of.AMFO >= m.o_amfo);
-
-      if (ot.AMFX == m.o_amfo) { //directly inside
-          assert ((ot != ct) && (ct.AMFX == m.c_amfx));
-          assert refOK(of,ot);
-          assert refOK(cf,ct);
-        } else  {
-          assert refOK(cf,ct);
-          assert (refOK(of,ot) ==> refOK(cf,ct));
-        }
-
-      assert (refOK(of,ot) ==> refOK(cf,ct));
-
-      } else {
-        assert ((v != k) && (v.AMFO >= m.c_amfx));  //inside & cloned
-
-        assert (refOK(of,ot) ==> refOK(cf,ct));
-      }
-        assert refOK(v,ct);
-        assert wexy_NO_builtin(i,j,m.m[i],m.m[j],m);
-                }
-//         else {
-//
-//
-//
-//       if (refDI(of,k)) {
-//
-//
-//       if (ot.AMFX == m.o_amfo) { //directly inside
-//           assert ((ot != ct) && (ct.AMFX == m.c_amfx));
-//           assert refOK(of,ot);
-//           assert refOK(cf,ct);
-//
-//         assume refOK(cf,k);
-//         }} else {
-//       if (refBI(of,ot)) {
-//         assume refOK(cf,ct);
-//        } else {
-//         assert not(refOK(of,ot));
-//         assert dexy_NO_builtin(i,j,m.m[i],m.m[j],m);
-//        }}}
-       }}
-
-
-assume dexy_NO_builtin(i,j,m.m[i],m.m[j],m);
-
-
-   } //end of FORALL statement
-
-// var i := k;  assert (forall j <- m'.m.Keys :: wexy_NO_builtin(i,j,m.m[i],m.m[j],m));
-// var j := k;  assert (forall i <- m'.m.Keys :: wexy_NO_builtin(i,j,m.m[i],m.m[j],m));
-
-  assume (forall i <- m.m.Keys, j <- m.m.Keys :: dexy_NO_builtin(i,j,m.m[i],m.m[j],m));
-
-} //done lemma KVscratchMonkey
-
-
-
-
-
-
-
-
-
-
-
-lemma kvdArmedStruggle(m' : Klon, k : Object, v : Object, of : Object, ot : Object, cf : Object, ct: Object, m : Klon)
-//refDI(k,ot) case
-
-  requires k !in m'.m.Keys
-  requires v !in m'.m.Values
-  requires m == subklonKV(m',k,v)
-
-  requires (of != ot)
-  requires GRURK: (of != ot)
-
-  requires (refDI(of,ot) && (of == k))
-
-  requires {of, ot} <= m.m.Keys
-  requires m.m[of] == cf
-  requires m.m[ot] == ct
-
-  requires k.Ready()
-  requires v.Ready()
-  requires forall k <- m'.m.Keys :: k.Ready() && m.m[k].Ready()
-
-  requires allmagic2(m')
-  requires magic2(k,v,m')
-//  ensures  allmagic2(m)
-
-  requires dexford4(m')
-
-  // ensures  dexy_NO_builtin(of,ot,cf,ct,m)
-  //  ensures  refOK(of,ot) ==> refOK(cf,ct)
-  {
-
-
-//     assert of != ot;
-//     assert (of == k) != (ot == k);
-//     //from here on, of one of and ot is k, the other is not
-
-//  if (refDI(of,ot) && (of == k)) {//refDI(k,ot)
-
-    assert of != ot by { reveal GRURK; }
-
-    // assert of.AMFO == ot.AMFX;  //by defn DI
-
-  // //  //  kdvDIKN(m', k, v, of, ot, cf, ct, m);
-
-//     if (k == v) {
-//       assert not(of.AMFO >= m.o_amfo); //k outside
-//       assert of == cf == v == k; //k outside
-//       // assert refOK(k,v);
-//       // assert ct == m.m[ot];
-//       // assert magic(ot,ct,m);
-//
-//       assert of.AMFO == ot.AMFX;  //ref defin DI
-//       assert of.AMFO != m.o_amfo;
-//
-//       assert not(of.AMFO >= m.o_amfo);
-//
-//       if (ot.AMFX == m.o_amfo) { //directly inside
-//           assert ((ot != ct) && (ct.AMFX == m.c_amfx));
-//           assert refOK(of,ot);
-//           assert refOK(cf,ct);
-//         } else  {
-//           assert refOK(cf,ct);
-//           assert (refOK(of,ot) ==> refOK(cf,ct));
-//         }
-//
-//       assert (refOK(of,ot) ==> refOK(cf,ct));
-      // }
-//      else {
-//         assert ((v != k) && (v.AMFO >= m.c_amfx));  //inside & cloned
-//
-//         assert (refOK(of,ot) ==> refOK(cf,ct));
-//       }
-//         assert refOK(v,ct);
-//         assert wexy_NO_builtin(of,ot,cf,ct,m);
-                }
-//     }
-//     }
-//
-//   }
-
-
-
-
-
-
-
-lemma kvdOTHER(m' : Klon, k : Object, v : Object, of : Object, ot : Object, cf : Object, ct: Object, m : Klon)
-//refDI(k,ot) case
-
-  requires k !in m'.m.Keys
-  requires v !in m'.m.Values
-  requires m == subklonKV(m',k,v)
-
-  requires {of, ot} <= m.m.Keys
-  requires m.m[of] == cf
-  requires m.m[ot] == ct
-
-  requires k.Ready()
-  requires v.Ready()
-  requires forall k <- m'.m.Keys :: k.Ready() && m.m[k].Ready()
-
-  requires allmagic2(m')
-  requires magic2(k,v,m')
-  ensures  allmagic2(m)
-
-  requires dexford4(m')
-
-  // ensures  dexy_NO_builtin(of,ot,cf,ct,m)
-  //  ensures  refOK(of,ot) ==> refOK(cf,ct)
-  {
-
-
-  }
-
-
-
-
-
-
-
-
-
-
-lemma {:isolate_assertions}
-NOT_ACTUALLY_FUCKED_OUTSIE_CANT_POUNT_IN(m' : Klon, f : Object, t : Object, o : Object, c : Object)
-//  requires o in m'.m.Keys
-//  requires m'.m[o] == c
-//  requires m'.o_amfo == o.AMFO
-//  requires m'.c_amfx == c.AMFO
-
- requires f.Ready()
- requires t.Ready()
- requires o.Ready()
- requires c.Ready()
-
- requires outside(f,o)
- requires  o != f
- requires inside(t,o)
- requires  t != o
- ensures   f != t
-
-  ensures not(refOK(f,t))
-{
-  /// AFTER ALL THIS FUCKING WORK
-  /// TURNS OUT TO VERIFY WITH... NOTHING.
-//   assert f.Ready(); assert t.Ready(); assert o.Ready();
-//
-//   assert not(f.AMFO >= o.AMFO); //outside(f,o)
-//   assert t.AMFO >= o.AMFO; //inside(t,o)
-//
-//   //  assert f != t;
-//   assert not(f.AMFO > o.AMFO);
-//   assert t.AMFO >= o.AMFO;
-//   assert t != o;
-//   AXIOMAMFOS(t,o);
-//   assert t.AMFO > o.AMFO;
-//   assert f != t;
-//
-// // assert refDI() case - f.AMFO != t.AMFX
-//
-// // assume t !in o.AMFO;
-//
-//
-//     assert t.AMFO == (t.AMFX + {t});
-//     assert t.AMFO > o.AMFO;
-//
-//     assert t.AMFX >= o.AMFO;
-//
-//
-//     if (f.AMFO == t.AMFX)
-//       {
-//         skip();
-//
-//
-//       }
-//
-//   // assert not(f.AMFO == t.AMFX);
-//   // assert not(refDI(f,t));
-//
-//
-//
-// //  assert not(refOK(f,t));
-// //  assert (f==t) || refBI(f,t) || refDI(f,t);
-//
-// // assert not(f == t);
-// // assert t.AMFO >= o.AMFO;
-// // AXIOMAMFOS(f,t);
-// // AXIOMAMFOS(f,o);
-// // AXIOMAMFOS(t,o);
-}
-
-
-
-
-
-lemma {:isolate_assertions} kvdNOTKK(m' : Klon, k : Object, v : Object, of : Object, ot : Object, cf : Object, ct: Object, m : Klon)
-
-  requires ((of != k) && (ot != k))
-
-  requires k !in m'.m.Keys
-  requires v !in m'.m.Values
-  requires m == subklonKV(m',k,v)
-
-  requires {of, ot} <= m.m.Keys
-  requires m.m[of] == cf
-  requires m.m[ot] == ct
-
-  requires k.Ready()
-  requires v.Ready()
-  requires forall k <- m'.m.Keys :: k.Ready() && m.m[k].Ready()
-
-  requires allmagic2(m')
-  requires magic2(k,v,m')
-  ensures  allmagic2(m)
-
-  requires dexford4(m')
-//  ensures  dexford4(m)
-
-  ensures  dexy_NO_builtin(of,ot,cf,ct,m)
-  ensures  refOK(of,ot) ==> refOK(cf,ct)
-{
-  //the following is there, and works, and is slower than nothing
-//   assert v == m.m[k];
-//   assert forall mm <- m'.m.Keys :: m'.m[mm]  == m.m[mm];
-//   assert forall mm <- m.m.Keys :: ((mm in m'.m.Keys) ==> (m'.m[mm] == m.m[mm]));
-//   assert m.m.Keys == m'.m.Keys + {k};
-//
-//    assert allmagic2(m');
-//    assert forall mm <- m'.m.Keys       :: magic2(mm, m.m[mm], m);
-//    assert magic2(k,v,m);
-//    assert forall mm <- {k}             :: magic2(mm, m.m[mm], m);
-//    assert forall mm <- m'.m.Keys + {k} :: magic2(mm, m.m[mm], m);
-//    assert forall mm <- m.m.Keys        :: magic2(mm, m.m[mm], m);
-//    assert allmagic2(m);
-}
-
-
-predicate kvdReqs(m' : Klon, k : Object, v : Object, of : Object, ot : Object, cf : Object, ct: Object, m : Klon)
-{
-  && k !in m'.m.Keys
-  && v !in m'.m.Values
-  && m == subklonKV(m',k,v)
-
-  && {of, ot} <= m.m.Keys
-  && m.m[of] == cf
-  && m.m[ot] == ct
-
-  && k.Ready()
-  && v.Ready()
-  && (forall k <- m'.m.Keys :: k.Ready() && m.m[k].Ready())
-
-  && allmagic2(m')
-  && magic2(k,v,m')
-
-  && dexford4(m')
-}
-
-
-lemma kvdEQKK(m' : Klon, k : Object, v : Object, of : Object, ot : Object, cf : Object, ct: Object, m : Klon)
-
-  requires (of == ot == k)
-
-  requires kvdReqs(m',k,v,of,ot,cf,ct,m)
-
-  ensures  allmagic2(m)
-
-  //requires dexford4(m')
-//  ensures  dexford4(m)
-
-  ensures refOK(of,ot)
-  ensures refOK(cf,ct)
-
-  ensures  dexy_NO_builtin(of,ot,cf,ct,m)
-  ensures  refOK(of,ot) ==> refOK(cf,ct)
-{}
-
-
-lemma kvdOO(m' : Klon, k : Object, v : Object, of : Object, ot : Object, cf : Object, ct: Object, m : Klon)
-
-  requires not(of.AMFO >= m'.o_amfo) //needs an o_o so we can write inside...
-  requires not(ot.AMFO >= m'.o_amfo) //needs an o_o so we can write inside...
-
-  requires kvdReqs(m',k,v,of,ot,cf,ct,m)
-
-  ensures  allmagic2(m)   //a bit slow
-
-//  ensures  dexford4(m)
-
-  ensures  dexy_NO_builtin(of,ot,cf,ct,m)
-  ensures  refOK(of,ot) ==> refOK(cf,ct)
-{
-   assert cf == of;
-   assert ct == ot;
-  allmagic2restored(m',k,v,m);
-}
-
-
-
-lemma {:isolate_assertions}  kvdOI(m' : Klon, k : Object, v : Object, of : Object, ot : Object, cf : Object, ct: Object, m : Klon, o : Object, c : Object)
-
-   requires of.Ready()
-   requires  o.Ready()
-   requires ot.Ready()
-
-  requires not(of.AMFO >= m'.o_amfo) //needs an o_o so we can write inside...
-  requires    (ot.AMFO >= m'.o_amfo) //needs an o_o so we can write inside...
-
-  requires kvdReqs(m',k,v,of,ot,cf,ct,m)
-
-  requires k !in m'.m.Keys
-  requires v !in m'.m.Values
-
-  requires o in m'.m.Keys
-  requires c == m'.m[o]
-  requires o.AMFO == m'.o_amfo
-  requires c.AMFO == m'.c_amfx
-
-  requires  o.AMFX == c.AMFX
-//wanted ensures  (o.AMFO - {o}) == (c.AMFO - {c})  //doesnt allow clone to be pushed down
-
-//KJX but outside stuff arent update by clone - should this be inside(of, o) ==> (refOK(of,ot) ==> refOK(cf,ct))
-//KJX but outside stuff arent update by clone - should this be inside(of, o) ==> (refOK(of,ot) ==> refOK(cf,ct))
-//KJX but outside stuff arent update by clone - should this be inside(of, o) ==> (refOK(of,ot) ==> refOK(cf,ct))
-
-//wanted but slows everything down
-// ensures  allmagic2(m)
-
-
-  //wanted but slows everything down
-  // ensures  dexy_NO_builtin(of,ot,cf,ct,m)
-  // ensures  refOK(of,ot) ==> refOK(cf,ct)
-{
-   assert of == cf by {
-    assert not( of.AMFO >= m'.o_amfo) by { assert   allmagic2(m'); }
-    }
-   assert of.Ready();
-   assert o.Ready();
-   assert ot.Ready();
-   assert outside(of,o); //&& (f != o) //unnecessary;
-   assert inside(ot,o);  //&& (t != o) //perhaps, perhaps, perhaps  //ieStrictlyInside;
-
-if (not(refOK(of,ot))) {
-    assert not(refOK(of,ot));
-    assert  refOK(of,ot) ==> refOK(cf,ct);
-    return;
-    }
-   assert refOK(of,ot);
-
-    INCOMING_REFS_OWNER_ONLY(of,ot,o);
-
-    assert ot == o;
-
-    assert cf == of;
-   assert m.m[ot] == ct;
-
-
-   assert refOK(of,ct);
-
-   assert ct.AMFO == m.c_amfx;
-   allmagic2restored(m',k,v,m);
-   assert allmagic2(m);
-
-    assert  dexy_NO_builtin(of,ot,cf,ct,m);
-    assert  refOK(of,ot) ==> refOK(cf,ct);
-}
-
-
-lemma kvdIO(m' : Klon, k : Object, v : Object, of : Object, ot : Object, cf : Object, ct: Object, o : Object, c : Object, m : Klon)
-
-  requires    (of.AMFO >= m'.o_amfo) //needs an o_o so we can write inside...
-  requires not(ot.AMFO >= m'.o_amfo) //needs an o_o so we can write inside...
-
-  requires kvdReqs(m',k,v,of,ot,cf,ct,m)
-/////////////////////////////////////////////////////////////////////////
-  requires k !in m'.m.Keys
-  requires v !in m'.m.Values
-
-  requires o in m'.m.Keys
-  requires c == m'.m[o]
-  requires o.AMFO == m'.o_amfo
-  requires c.AMFO == m'.c_amfx
-  requires cf.AMFB >= of.AMFB
-
-  requires  o.AMFX == c.AMFX
-  ensures  (o.AMFO - {o}) == (c.AMFO - {c})  //doesnt allow clone to be pushed down
-
-//KJX but outside stuff arent update by clone - should this be inside(of, o) ==> (refOK(of,ot) ==> refOK(cf,ct))
-//KJX but outside stuff arent update by clone - should this be inside(of, o) ==> (refOK(of,ot) ==> refOK(cf,ct))
-//KJX but outside stuff arent update by clone - should this be inside(of, o) ==> (refOK(of,ot) ==> refOK(cf,ct))
-
-/////////////////////////////////////////////////////////////////////////
-//corret but slow ensures  allmagic2(m)
-//
-  //  ensures  dexy_NO_builtin(of,ot,cf,ct,m)
-  //  ensures  refOK(of,ot) ==> refOK(cf,ct)
-{
-  assert magic2(k,v,m');
-  assert ot == ct;
-//
-  if (refOK(of,ot)) {
-    assert of != ot;
-    assert not(refDI(of,ot));
-    assert refBI(of,ot);
-    assert of.AMFB >= ot.AMFX;
-
-    assert cf.AMFB >= of.AMFB;
-    assert ct.AMFX == ot.AMFX;
-    assert cf.AMFB >= ct.AMFX;
-    assert refBI(cf,ct);
-    assert refOK(cf,ct);
-  }
-
-   allmagic2restored(m',k,v,m);
-}
-
-
-lemma {:isolate_assertions} kvdII(m' : Klon, k : Object, v : Object, of : Object, ot : Object, cf : Object, ct: Object, m : Klon)
-
-  requires kvdReqs(m',k,v,of,ot,cf,ct,m)
-
-  requires forall k <- m'.m.Keys :: k.owner <= m'.m.Keys   //IN-KLON
-  requires forall k <- m'.m.Keys :: k.AMFO  <= m'.m.Keys   //IN-KLON
-  requires m'.o_amfo <= m'.m.Keys  //IN-KLON
-
-  requires forall o <- m.m.Keys :: && (o.AMFO <= m.m.Keys) && (o.bound <= m.m.Keys) && (o.owner <= m.m.Keys) && (o.ntrnl <= m.m.Keys) //IN-KLON
-
-  requires k.owner <= m.m.Keys   //IN-KLON
-  requires k.AMFO  <= m.m.Keys   //IN-KLON
-  requires magic3(k,v,m)
-
-  requires dante(of,m)
-  requires dante(ot,m)
-  requires dante(cf,m)
-  requires dante(ct,m)
-
-  requires allmagic2(m')
-  requires allmagic3(m')
-
-  requires    (of.AMFO >= m'.o_amfo) //needs an o_o so we can write inside...
-  requires    (ot.AMFO >= m'.o_amfo)
-   //this means of & ot are both inside: k will be one or other of them...
-
-  // ensures  allmagic2(m) //working?? but tricky
-  // ensures  allmagic3(m)
-
-  requires dexford4(m')
-//  ensures  dexford4(m)
-//
-//   ensures  dexy_NO_builtin(of,ot,cf,ct,m)
-//   ensures  refOK(of,ot) ==> refOK(cf,ct)
-{
-  assert kvdReqs(m',k,v,of,ot,cf,ct,m);
-
-  assert
-  && {of, ot} <= m.m.Keys
-  && m.m[of] == cf
-  && m.m[ot] == ct
-  ;
-
-  assert m.from(m');
-  assert magic3(k,v,m);
-
-  allmagic2restored(m',k,v,m);
-  allmagic3restored(m',k,v,m);
-
-
-  assert allmagic3(m);
-
-  assert k in m.m.Keys;
-  assert v in m.m.Values;
-  assert m.m[k] == v;
-  assert m.o_amfo <= m.m.Keys;
-  assert k.owner <= m.m.Keys;
-  assert k.AMFO  <= m.m.Keys;
-
-  assert {k, of, ot} <= m.m.Keys;
-  assert {v, cf, ct} <= m.m.Values;
-
-  // assert oxy_NO_builtin(of,ot,cf,ct,m');
-  // assert(inside(of,ot) ==> inside(cf,ct));
-     if (refOK(of,ot)) {
-
-magic3preservesOwnership(m);
-
-//assert forall i <- m.m.Keys, j <- m.m.Keys ::  (oxy_NO_builtin(i,j,m.m[i],m.m[j],m));
-assert forall i <- m.m.Keys, j <- m.m.Keys :: (inside(i,j) ==> inside(m.m[i],m.m[j]));
-
-assert forall i <- m.m.Keys, j <- m.m.Keys :: (inside(i,j) ==> inside(m.m[i],m.m[j]));
-
-assert M3K: magic3(k,v,m);
-assert M3F: magic3(of,cf,m);
-assert M3T: magic3(ot,ct,m);
-
-  assert
-  && {of, ot} <= m.m.Keys
-  && m.m[of] == cf
-  && m.m[ot] == ct
-  ;
-
-fuckenHell3(of,ot,cf,ct,m);
-
-
-
-// assert (inside(of,ot) ==> inside(cf,ct));
-// //
-// //     //continue here!
-// //     //continue here!
-// //     //continue here!
-// //     //continue here!
-// // //
-// // //         assert (of.AMFO >= m.o_amfo) && (ot.AMFO >= m.o_amfo);
-// // //         assert cf.AMFO >= m.c_amfx;
-// // //         assert ct.AMFO >= m.c_amfx;
-//
-//   if (of == ot) {
-//     assert refOK(of,ot);
-//     assert refOK(cf,ct);
-//     return;
-//   }
-//
-//   if (refDI(of,ot)) {
-//     assert refOK(of,ot);
-//     assert (of.AMFO == ot.AMFX);
-//     assert magic3(of,cf,m) by { reveal M3F; }
-//     assert tragic3(of,m) == cf.AMFO;
-//     assert cf.Ready();
-//     assert magic3(ot,ct,m) by { reveal M3T; }
-//     assert tragic3(ot,m) == ct.AMFO;
-//     assert ct.Ready();
-//     assert ct.AMFX == ct.AMFO - {ct};
-//
-//
-//   //  assert refOK(cf,ct);
-//     return;
-//   }
-//
-//   if (refBI(of,ot)) {
-//     assert refOK(of,ot);
-//     assert magic3(of,cf,m) by { reveal M3F; }
-//     assert magic3(ot,ct,m) by { reveal M3T; }
-//   //  assert refOK(cf,ct);
-//     return;
-//    }
-//
-//    assert {:contradiction} not(refOK(of,ot));
-//    assert {:contradiction} false;
-//
-// //
-//    }
-// //
-     }
-//////////////////////////////t  assert refOK(of,ot) ==> refOK(cf,ct);
-}
-
-
-
-
-lemma {:verify false}  //FUCKED2
-kdvDIKN(m' : Klon, k : Object, v : Object, of : Object, ot : Object, cf : Object, ct: Object, m : Klon)
-
-  requires (refDI(of,ot) && (of == k))
-  requires refDI(k,ot)
-
-  requires not((of != k) && (ot != k))
-  requires not(of == ot)
-
-  requires k !in m'.m.Keys
-  requires v !in m'.m.Values
-  requires m == subklonKV(m',k,v)
-
-  requires {of, ot} <= m.m.Keys
-  requires m.m[of] == cf
-  requires m.m[ot] == ct
-
-  requires k.Ready()
-  requires v.Ready()
-  requires forall k <- m'.m.Keys :: k.Ready() && m.m[k].Ready()
-
-  requires allmagic2(m')
-  requires magic2(k,v,m')
-  ensures  allmagic2(m)
-
-  requires dexford4(m')
-
-  ensures  dexy_NO_builtin(of,ot,cf,ct,m)
-  ensures  refOK(of,ot) ==> refOK(cf,ct)
-{
-    assert of != ot;
-    assert (of == k) != (ot == k);
-    assert ot != k;
-    assert of.AMFO == ot.AMFX;  //by defn DI
-
-    if (k == v) {
-      assert not(of.AMFO >= m.o_amfo); //k outside
-      assert of == cf == v == k; //k outside
-      // assert refOK(k,v);
-      // assert ct == m.m[ot];
-      // assert magic(ot,ct,m);
-
-      assert of.AMFO == ot.AMFX;  //ref defin DI
-      assert of.AMFO != m.o_amfo;
-
-      assert not(of.AMFO >= m.o_amfo);
-
-      if (ot.AMFX == m.o_amfo) { //directly inside
-          assert ((ot != ct) && (ct.AMFX == m.c_amfx));
-          assert refOK(of,ot);
-          assert refOK(cf,ct);
-        } else  {
-          assert refOK(cf,ct);
-          assert (refOK(of,ot) ==> refOK(cf,ct));
-        }
-
-      assert (refOK(of,ot) ==> refOK(cf,ct));
-
-      } else {
-        assert ((v != k) && (v.AMFO >= m.c_amfx));  //inside & cloned
-
-        assert (refOK(of,ot) ==> refOK(cf,ct));
-      }
-        assert refOK(v,ct);
-}
-
-
-
-
-
-
-
-
-
-
-
-
-
-
-
-
-
-
-
-
-
-
-
-
-
-
-//extrabit#1
-//         if (ot.AMFO >= m.o_amfo) //inside
-//          { assert ((ot != ct) && (ct.AMFO >= m.c_amfx));
-//            assert refOK(of,ot);
-//            assert refOK(cf,ct); }
-
-
-
-lemma {:verify false} KVwexy(m' : Klon, k : Object, v : Object, m : Klon)
-  requires k !in m'.m.Keys
-  requires v !in m'.m.Values
-  requires m == subklonKV(m',k,v)
-
-  requires allmagic(m')
-
-
-  requires magic(k,v,m')
-  ensures  allmagic(m)
-
-  requires cexford4(m')
-  ensures  cexford4(m)
-  {
-
-assert (forall i <- m'.m.Keys, j <- m'.m.Keys :: cexy_NO_builtin(i,j,m.m[i],m.m[j],m));
-assert m.m.Keys == m'.m.Keys + {k};
-
-assert allmagic(m);
-
-assert m.m[k] == v;
-assert magic(k,v,m);
-
-
-forall i <- m.m.Keys, j <- m.m.Keys
-   ensures  wexy_NO_builtin(i,j,m.m[i],m.m[j],m)
-   {
-     var of := i; var ot := j;  var cf := m.m[i]; var ct := m.m[j];
-
-  if (not(of.AMFO >= m.o_amfo))  //from outside
-    {
-      if (not(ot.AMFO >= m.o_amfo)) //both outside
-       {
-        assert (not(of.AMFO >= m.o_amfo)) && (not(ot.AMFO >= m.o_amfo));
-        assert of == cf;
-        assert ot == ct;
-        assert refOK(of,ot) ==> refOK(cf,ct);
-        } else {
-        // //from outside to inside...
-        assert (not(of.AMFO >= m.o_amfo)) && (ot.AMFO >= m.o_amfo);
-        assert of == cf;
-        assert ct.AMFO >= m.c_amfx;
-
-        if ((of == k) && (ot == k))
-          {
-            // assert k == of == ot == cf == cf == v;
-            // assert of.AMFO == ot.AMFO;
-            // assert {:contradiction} not( (not(of.AMFO >= m.o_amfo)) && (ot.AMFO >= m.o_amfo) );
-            // assert {:contradiction} not( refOK(of,ot));
-            // assert {:contradiction} false;
-            assert refOK(of,ot) ==> refOK(cf,ct); //staggering
-          }
-        else if ((of == k) && (ot != k))
-         {
-            assert of == cf;
-            assert of.AMFO == cf.AMFO;
-            assert not(of.AMFO >= m.o_amfo);
-            assert ot.AMFO >= m.o_amfo;
-            if (ot.AMFO > m.o_amfo) { assert refOK(of,ot); }
-            assert ct.AMFO >= m.c_amfx;
-            //assert magic(k,v,m);
-            assert refOK(of,ot) ==> refOK(cf,ct);
-          }
-        else if ((of != k) && (ot == k))
-         {
-            assert of == cf;
-            assert magic(k,v,m);
-            assert refOK(of,ot) ==> refOK(cf,ct);
-        } else {
-            assert refOK(of,ot) ==> refOK(cf,ct);
-        }
-
-        assert refOK(of,ot) ==> refOK(cf,ct);
-        }
-    } else {
-        assume wexy_NO_builtin(i,j,m.m[i],m.m[j],m);
-    }
-   }
-
-
-
-// var i := k;  assert (forall j <- m'.m.Keys :: wexy_NO_builtin(i,j,m.m[i],m.m[j],m));
-//
-// var j := k;  assert (forall i <- m'.m.Keys :: wexy_NO_builtin(i,j,m.m[i],m.m[j],m));
-
-  assert (forall i <- m.m.Keys, j <- m.m.Keys :: wexy_NO_builtin(i,j,m.m[i],m.m[j],m));
-
-}//done lemma VERIFY FALSE  KVwexy
-
-
-// assert (of.AMFO >= m.o_amfo);  //from inside
-//
-//
-//       (if (not(ot.AMFO >= m.o_amfo)) then (
-//         //from inside to outside
-//         assert (of.AMFO >= m.o_amfo) && (not(ot.AMFO >= m.o_amfo));
-//         assert cf.AMFO >= m.c_amfx;
-//         assert ot == ct;
-//         refOK(of,ot) ==> refOK(cf,ct)
-//       ) else (
-//         //both inside
-//         assert (of.AMFO >= m.o_amfo) && (ot.AMFO >= m.o_amfo);
-//         assert cf.AMFO >= m.c_amfx;
-//         assert ct.AMFO >= m.c_amfx;
-//         refOK(of,ot) ==> refOK(cf,ct)))
-//
-
-
-
-
-
-//
-//
-// assert
-//  forall i <- m.m.Keys, j <- m.m.Keys ::
-// //wexynobuiltin
-//   (var of := i; var ot := j;  var cf := m.m[i]; var ct := m.m[j];
-//
-//
-//
-//   if (not(of.AMFO >= m.o_amfo))
-//     then //from outside
-//       (if (not(ot.AMFO >= m.o_amfo)) then (
-//         //both outside
-//         assert (not(of.AMFO >= m.o_amfo)) && (not(ot.AMFO >= m.o_amfo));
-//         assert of == cf;
-//         assert ot == ct;
-//         refOK(of,ot) ==> refOK(cf,ct)
-//       ) else (
-//         //from outside to inside...
-//         assert (not(of.AMFO >= m.o_amfo)) && (ot.AMFO >= m.o_amfo);
-//         assert of == cf;
-//         assert ct.AMFO >= m.c_amfx;
-//         refOK(of,ot) ==> refOK(cf,ct)))
-//     else //from inside
-//       (if (not(ot.AMFO >= m.o_amfo)) then (
-//         //from inside to outside
-//         assert (of.AMFO >= m.o_amfo) && (not(ot.AMFO >= m.o_amfo));
-//         assert cf.AMFO >= m.c_amfx;
-//         assert ot == ct;
-//         refOK(of,ot) ==> refOK(cf,ct)
-//       ) else (
-//         //both inside
-//         assert (of.AMFO >= m.o_amfo) && (ot.AMFO >= m.o_amfo);
-//         assert cf.AMFO >= m.c_amfx;
-//         assert ct.AMFO >= m.c_amfx;
-//         refOK(of,ot) ==> refOK(cf,ct)))
-//
-//
-//
-//   );
-//
-//
-
-
-
-
-
-
-
-
-predicate {:isolate_assertions} oxy_NO_builtin(of : Object, ot : Object, cf : Object, ct: Object, m : Klon) : ( rv : bool )
-  requires {of, ot} <= m.m.Keys
-  requires m.m[of] == cf
-  requires m.m[ot] == ct
-
-  //requires allmagic(m)
-  // requires magic2(of,cf,m)
-  // requires magic2(ot,ct,m)
-
-//  requires (forall x <- m.m.Keys :: (not(x.AMFO >= m.o_amfo) <==> (m.m[x] == x)))
-  //seems not to requires ANY other constraints than this one...
-//
-//   requires (of != cf) ==> (cf.AMFO >= m.c_amfx)
-//   requires (ot != ct) ==> (ct.AMFO >= m.c_amfx)
-
-
-  ensures rv == (inside(of,ot) ==> inside(cf,ct))
-{
-(inside(of,ot) ==> inside(cf,ct))
-}
-
-
-
-
-
-
-
-
-
-
-
-
-
-
-
-
-
-
-
-
-
-predicate wexy(of : Object, ot : Object, cf : Object, ct: Object, m : SuperKlon) : ( rv : bool )
-//note doesnt requrie Valid???
-// this Kklon has wexford2()  BUILT IN@!!A
-  requires {of, ot} <= m.m.Keys
-  requires m.m[of] == cf
-  requires m.m[ot] == ct
-
-  requires (forall x <- m.m.Keys :: (not(x.AMFO >= m.o_amfo) <==> (m.m[x] == x)))
-
-  requires (of != cf) ==> (cf.AMFO >= m.c_amfx)
-  requires (ot != ct) ==> (ct.AMFO >= m.c_amfx)
-
-  ensures rv == (refOK(of,ot) ==> refOK(cf,ct))
-{
-
-  // 25DEC 2024 - starting on the 2x2 version inside/outside of ,ot cases
-  //
-  if (not(of.AMFO >= m.o_amfo))
-    then //from outside
-      (if (not(ot.AMFO >= m.o_amfo)) then (
-        //both outside
-        assert (not(of.AMFO >= m.o_amfo)) && (not(ot.AMFO >= m.o_amfo));
-        assert of == cf;
-        assert ot == ct;
-        refOK(of,ot) ==> refOK(cf,ct)
-      ) else (
-        //from outside to inside...
-        assert (not(of.AMFO >= m.o_amfo)) && (ot.AMFO >= m.o_amfo);
-        assert of == cf;
-        assert ct.AMFO >= m.c_amfx;
-        refOK(of,ot) ==> refOK(cf,ct)))
-    else //from inside
-      (if (not(ot.AMFO >= m.o_amfo)) then (
-        //from inside to outside
-        assert (of.AMFO >= m.o_amfo) && (not(ot.AMFO >= m.o_amfo));
-        assert cf.AMFO >= m.c_amfx;
-        assert ot == ct;
-        refOK(of,ot) ==> refOK(cf,ct)
-      ) else (
-        //both inside
-        assert (of.AMFO >= m.o_amfo) && (ot.AMFO >= m.o_amfo);
-        assert cf.AMFO >= m.c_amfx;
-        assert ct.AMFO >= m.c_amfx;
-        refOK(of,ot) ==> refOK(cf,ct)))
-}
-
-
-
-
-predicate wexy_NO_builtin(of : Object, ot : Object, cf : Object, ct: Object, m : Klon) : ( rv : bool )
-
-  // requires {of, ot} <= m.m.Keys
-  // requires m.m[of] == cf
-  // requires m.m[ot] == ct
-
-  //requires allmagic(m)
-  requires magic2(of,cf,m)
-  requires magic2(ot,ct,m)
-
-//  requires (forall x <- m.m.Keys :: (not(x.AMFO >= m.o_amfo) <==> (m.m[x] == x)))
-  //seems not to requires ANY other constraints than this one...
-//
-//   requires (of != cf) ==> (cf.AMFO >= m.c_amfx)
-//   requires (ot != ct) ==> (ct.AMFO >= m.c_amfx)
-
-
-  ensures rv == (refOK(of,ot) ==> refOK(cf,ct))
-{
-
-  // 25DEC 2024 - starting on the 2x2 version inside/outside of ,ot cases
-  //
-  if (not(of.AMFO >= m.o_amfo))
-    then //from outside
-      (if (not(ot.AMFO >= m.o_amfo)) then (
-        //both outside
-        assert (not(of.AMFO >= m.o_amfo)) && (not(ot.AMFO >= m.o_amfo));
-        assert of == cf;
-        assert ot == ct;
-        refOK(of,ot) ==> refOK(cf,ct)
-      ) else (
-        //from outside to inside...
-        assert (not(of.AMFO >= m.o_amfo)) && (ot.AMFO >= m.o_amfo);
-        assert of == cf;
-        assert ct.AMFO >= m.c_amfx;
-        refOK(of,ot) ==> refOK(cf,ct)))
-    else //from inside
-      (if (not(ot.AMFO >= m.o_amfo)) then (
-        //from inside to outside
-        assert (of.AMFO >= m.o_amfo) && (not(ot.AMFO >= m.o_amfo));
-        assert cf.AMFO >= m.c_amfx;
-        assert ot == ct;
-        refOK(of,ot) ==> refOK(cf,ct)
-      ) else (
-        //both inside
-        assert (of.AMFO >= m.o_amfo) && (ot.AMFO >= m.o_amfo);
-        assert cf.AMFO >= m.c_amfx;
-        assert ct.AMFO >= m.c_amfx;
-        refOK(of,ot) ==> refOK(cf,ct)))
-}
-
-
-
-
-predicate dexy(of : Object, ot : Object, cf : Object, ct: Object, m : SuperKlon) : ( rv : bool )
-//  requires wexford3(m)
-/// HMM doesit still work?
-// agan doesn't need Valid??
-// this Kklon has wexford2()  BUILT IN !!A
-  // requires {of, ot} <= m.m.Keys
-  // requires m.m[of] == cf
-  // requires m.m[ot] == ct
-
-  // requires (forall x <- m.m.Keys :: (not(x.AMFO >= m.o_amfo) <==> (m.m[x] == x)))
-
-  ensures rv == (refOK(of,ot) ==> refOK(cf,ct))
-{
-
-  // 25DEC 2024 - version done by case analysis of the refOK(of,ot)
-  //
-
-  if (of == ot) then (
-    assert refOK(of,ot);
-    refOK(cf,ct)) else (
-  if (refDI(of,ot)) then (
-    assert refOK(of,ot);
-    refOK(cf,ct)) else (
-  if (refBI(of,ot)) then (
-    assert refOK(of,ot);
-    refOK(cf,ct)
-  ) else (
-    assert not(refOK(of,ot));
-    true)))
-}
-
-
-
-predicate dexy_NO_builtin(of : Object, ot : Object, cf : Object, ct: Object, m : Klon) : ( rv : bool )
-//no builtin constraints version
-  // requires {of, ot} <= m.m.Keys
-  // requires m.m[of] == cf
-  // requires m.m[ot] == ct
-
-  // requires (forall x <- m.m.Keys :: (not(x.AMFO >= m.o_amfo) <==> (m.m[x] == x)))
-
-  ensures rv == (refOK(of,ot) ==> refOK(cf,ct))
-{
-
-  // 25DEC 2024 - version done by case analysis of the refOK(of,ot)
-  //
-
-  if (of == ot) then (
-    assert refOK(of,ot);
-    refOK(cf,ct)) else (
-  if (refDI(of,ot)) then (
-    assert refOK(of,ot);
-    refOK(cf,ct)) else (
-  if (refBI(of,ot)) then (
-    assert refOK(of,ot);
-    refOK(cf,ct)
-  ) else (
-    assert not(refOK(of,ot));
-    true)))
-}
-
-
-
-lemma compare_NO_builtin(of : Object, ot : Object, cf : Object, ct: Object, m : Klon)
-
-  requires allmagic2(m)
-
-  requires {of, ot} <= m.m.Keys
-  requires m.m[of] == cf
-  requires m.m[ot] == ct
-
-//   requires (forall x <- m.m.Keys :: (not(x.AMFO >= m.o_amfo) <==> (m.m[x] == x)))
-//
-//   requires (of != cf) ==> (cf.AMFO >= m.c_amfx)
-//   requires (ot != ct) ==> (ct.AMFO >= m.c_amfx)
-
-  ensures  dexy_NO_builtin(of,ot,cf,ct,m)  ==> wexy_NO_builtin(of,ot,cf,ct,m)
-  ensures  dexy_NO_builtin(of,ot,cf,ct,m) <==  wexy_NO_builtin(of,ot,cf,ct,m)
-  ensures  dexy_NO_builtin(of,ot,cf,ct,m) <==> wexy_NO_builtin(of,ot,cf,ct,m)
-
-  ensures  dexy_NO_builtin(of,ot,cf,ct,m)  ==> cexy_NO_builtin(of,ot,cf,ct,m)
-  ensures  dexy_NO_builtin(of,ot,cf,ct,m) <==  cexy_NO_builtin(of,ot,cf,ct,m)
-  ensures  dexy_NO_builtin(of,ot,cf,ct,m) <==> cexy_NO_builtin(of,ot,cf,ct,m)
-
-  ensures  wexy_NO_builtin(of,ot,cf,ct,m)  ==> cexy_NO_builtin(of,ot,cf,ct,m)
-  ensures  wexy_NO_builtin(of,ot,cf,ct,m) <==  cexy_NO_builtin(of,ot,cf,ct,m)
-  ensures  dexy_NO_builtin(of,ot,cf,ct,m) <==> cexy_NO_builtin(of,ot,cf,ct,m)
-
-  ensures  dexy_NO_builtin(of,ot,cf,ct,m)
-      == cexy_NO_builtin(of,ot,cf,ct,m)
-      == wexy_NO_builtin(of,ot,cf,ct,m)
-
-{
-//
-// assert  dexy_NO_builtin(of,ot,cf,ct,m) <==> wexy_NO_builtin(of,ot,cf,ct,m);
-// assert  dexy_NO_builtin(of,ot,cf,ct,m) <==> cexy_NO_builtin(of,ot,cf,ct,m);
-// assert  dexy_NO_builtin(of,ot,cf,ct,m) <==> cexy_NO_builtin(of,ot,cf,ct,m);
-// assert  dexy_NO_builtin(of,ot,cf,ct,m)
-//       == cexy_NO_builtin(of,ot,cf,ct,m)
-//       == wexy_NO_builtin(of,ot,cf,ct,m);
-
-}
-
-predicate cexy_NO_builtin(of : Object, ot : Object, cf : Object, ct: Object, m : Klon)
-//
-//   requires {of, ot} <= m.m.Keys
-//   requires m.m[of] == cf
-//   requires m.m[ot] == ct
-
-{
-   refOK(of,ot) ==> refOK(cf,ct)
-}
-
-predicate magic3(k : Object, v : Object, m : Klon) : ( rv : bool )
-//see allmagic3 for why k & v must be in m already
-  requires k in m.m.Keys
-  requires v in m.m.Values
-  requires m.m[k] == v
-  requires m.o_amfo <= m.m.Keys   //IN-KLON
-  requires k.owner <= m.m.Keys   //IN-KLON
-  requires k.AMFO  <= m.m.Keys   //IN-KLON
-  reads m.oHeap`fields, m.oHeap`fieldModes
-  reads m.ns`fields, m.ns`fieldModes
-{
-  var CXTRA := m.c_amfx - mapThruKlon(m.o_amfo, m);
-  var OXTRA := mapThruKlon(m.o_amfo, m) - m.c_amfx;
-
-assert  mapThruKlon(m.o_amfo, m) - OXTRA + CXTRA == m.c_amfx;
-
-///KJX continue from here - needs to be done in parallel for owner & AMFO!
-///KJX continue from here - needs to be done in parallel for owner & AMFO!
-///KJX continue from here - needs to be done in parallel for owner & AMFO!
-
-  && (v.AMFO == (mapThruKlon(k.AMFO, m) - OXTRA + CXTRA )) //and this one???
-}
-
-
-function  tragic3(k : Object, m : Klon) : Owner
-  requires k in m.m.Keys
-  // requires v in m.m.Values
-  // requires m.m[k] == v
-  requires m.o_amfo <= m.m.Keys   //IN-KLON
-  requires k.owner <= m.m.Keys   //IN-KLON
-  requires k.AMFO  <= m.m.Keys   //IN-KLON
-  reads m.oHeap`fields, m.oHeap`fieldModes
-  reads m.ns`fields, m.ns`fieldModes
-{
-  var CXTRA := m.c_amfx - mapThruKlon(m.o_amfo, m);
-  var OXTRA := mapThruKlon(m.o_amfo, m) - m.c_amfx;
-
-assert  (mapThruKlon(m.o_amfo, m) - OXTRA + CXTRA) == m.c_amfx;
-
-///KJX continue from here - needs to be done in parallel for owner & AMFO!
-///KJX continue from here - needs to be done in parallel for owner & AMFO!
-///KJX continue from here - needs to be done in parallel for owner & AMFO!
-
-  (mapThruKlon(k.AMFO, m) - OXTRA + CXTRA ) //and this one??
-}
-
-
-
-lemma  magic3tragic3(k : Object, v : Object, m : Klon)
-  requires k in m.m.Keys
-  requires v in m.m.Values
-  requires m.m[k] == v
-  requires m.o_amfo <= m.m.Keys   //IN-KLON
-  requires k.owner <= m.m.Keys   //IN-KLON
-  requires k.AMFO  <= m.m.Keys   //IN-KLON
-  requires magic3(k,v,m)
-  ensures (
-    var mTKoA := mapThruKlon(m.o_amfo, m);
-    var CXTRA := m.c_amfx - mTKoA;
-    var OXTRA := mTKoA - m.c_amfx;
-    && ((mTKoA - OXTRA + CXTRA) == m.c_amfx)
-    && (v.AMFO == tragic3(k,m))
-  )
-{
-    var mTKoA := mapThruKlon(m.o_amfo, m);
-    var CXTRA := m.c_amfx - mTKoA;
-    var OXTRA := mTKoA - m.c_amfx;
-    assert
-      && ((mTKoA - OXTRA + CXTRA) == m.c_amfx)
-      && (v.AMFO == tragic3(k,m))
-      ;
-}
-
-lemma magic3sanity(m : Klon, o : Object, c : Object)
-  requires o.AMFO == m.o_amfo
-  requires c.AMFO == m.c_amfx
-  requires o in m.m.Keys
-  requires c in m.m.Values
-  requires m.m[o] == c
-//see allmagic3 for why k & v must be in m already
-  requires forall k <- m.m.Keys :: k.owner <= m.m.Keys   //IN-KLON
-  requires forall k <- m.m.Keys :: k.AMFO  <= m.m.Keys   //IN-KLON
-  requires allmagic3(m)
-  requires m.o_amfo <= m.m.Keys
-  requires m.c_amfx == m.m[o].AMFO
-  ensures  magic3(o, c, m)
-{}
-
-
-predicate allmagic3(m : Klon)
-  requires forall k <- m.m.Keys :: k.owner <= m.m.Keys   //IN-KLON
-  requires forall k <- m.m.Keys :: k.AMFO  <= m.m.Keys   //IN-KLON
-  requires m.o_amfo <= m.m.Keys   //IN-KLON
-
-  reads m.oHeap`fields, m.oHeap`fieldModes
-  reads m.ns`fields, m.ns`fieldModes
-{
-
-  forall x <- m.m.Keys :: magic3(x,m.m[x],m)
-}
-
-lemma allmagic3restored(m' : Klon, k : Object, v : Object, m : Klon)
-  requires k !in m'.m.Keys
-  requires v !in m'.m.Values
-  requires forall k <- m'.m.Keys :: k.owner <= m'.m.Keys   //IN-KLON
-  requires forall k <- m'.m.Keys :: k.AMFO  <= m'.m.Keys   //IN-KLON
-  requires m'.o_amfo <= m'.m.Keys   //IN-KLON
-  requires allmagic3(m')
-  requires m == subklonKV(m',k,v)
-
-  requires k.owner <= m.m.Keys   //IN-KLON
-  requires k.AMFO  <= m.m.Keys   //IN-KLON
-  requires magic3(k,v,m)
-
-  ensures  allmagic3(m)
-{
-  assert v == m.m[k];
-  assert forall mm <- m'.m.Keys :: m'.m[mm]  == m.m[mm];
-  assert forall mm <- m.m.Keys :: ((mm in m'.m.Keys) ==> (m'.m[mm] == m.m[mm]));
-  assert m.m.Keys == m'.m.Keys + {k};
-
-   assert allmagic3(m');
-   assert forall mm <- m'.m.Keys       :: magic3(mm, m.m[mm], m);
-   assert magic3(k,v,m);
-   assert forall mm <- {k}             :: magic3(mm, m.m[mm], m);
-   assert forall mm <- m'.m.Keys + {k} :: magic3(mm, m.m[mm], m);
-   assert forall mm <- m.m.Keys        :: magic3(mm, m.m[mm], m);
-   assert allmagic3(m);
-}
-
-
-lemma magic3preservesOwnership(m : Klon)
-  requires forall k <- m.m.Keys :: k.owner <= m.m.Keys   //IN-KLON
-  requires forall k <- m.m.Keys :: k.AMFO  <= m.m.Keys   //IN-KLON
-  requires m.o_amfo <= m.m.Keys
-  requires allmagic3(m)
-  ensures forall i <- m.m.Keys, j <- m.m.Keys ::  (oxy_NO_builtin(i,j,m.m[i],m.m[j],m))
-  {
-assert forall i <- m.m.Keys :: magic3(i,m.m[i],m);
-
-forall i <- m.m.Keys, j <- m.m.Keys
-  ensures (oxy_NO_builtin(i,j,m.m[i],m.m[j],m))
-  {
-    if (i == j) { return; }
-    if (inside(i,j)) {
-        assert i.AMFO >= j.AMFO;
-        assert magic3(i,m.m[i], m);
-        assert magic3(j,m.m[j], m);
-    }
-    assert (oxy_NO_builtin(i,j,m.m[i],m.m[j],m));
-  }
-  }
-
-
-function supertragic(k : Owner, m : Klon) : Owner
-  requires m.o_amfo <= m.m.Keys   //IN-KLON
-  requires k <= m.m.Keys
-  reads m.oHeap`fields, m.oHeap`fieldModes
-  reads m.ns`fields, m.ns`fieldModes
-{
-  var CXTRA := m.c_amfx - mapThruKlon(m.o_amfo, m);
-  var OXTRA := mapThruKlon(m.o_amfo, m) - m.c_amfx;
-
-  (mapThruKlon(k,m) - OXTRA + CXTRA )
-}
-
-//or should this take another parameter for v?
-predicate tragicallyhip(o : Object, m : Klon)
-  requires m.o_amfo <= m.m.Keys   //IN-KLON
-  requires m.m.Keys >= o.ntrnl > o.owner >= o.bound
-  requires m.m.Keys >= o.AMFO  > o.AMFX  >= o.AMFB
-  requires o in m.m.Keys
-  reads m.oHeap`fields, m.oHeap`fieldModes
-  reads m.ns`fields, m.ns`fieldModes
-   reads o
-{
-  var c := m.m[o];
-
-  && (c.bound == supertragic(o.bound, m))
-  && (c.AMFB  == supertragic(o.AMFB , m))
-  && (c.owner == supertragic(o.owner, m))
-  && (c.AMFX  == supertragic(o.AMFX , m))
-  && (c.ntrnl == supertragic(o.ntrnl, m))
-  && (c.AMFO  == supertragic(o.AMFO , m))
-}
-
-opaque predicate acertainratio(o : Object, m : Klon)
-{
-  reveal o.Ready();
-  && (m.o_amfo <= m.m.Keys)   //IN-KLON
-  && (m.m.Keys >= o.ntrnl > o.owner >= o.bound)
-  && (m.m.Keys >= o.AMFO  > o.AMFX  >= o.AMFB)
-  && (o in m.m.Keys)
-  && (o.Ready())
-}
-
-
-opaque predicate allcertainratio(m : Klon)
-{
-  forall o <- m.m.Keys :: acertainratio(o,m)
-}
-
-
-lemma fked1(o1 : Object, o2 : Object, m : Klon)
-  requires m.o_amfo <= m.m.Keys   //IN-KLON
-
-  requires m.m.Keys >= o1.ntrnl > o1.owner >= o1.bound
-  requires m.m.Keys >= o1.AMFO  > o1.AMFX  >= o1.AMFB
-  requires o1 in m.m.Keys
-  requires o1.Ready()
-
-  requires m.m.Keys >= o2.ntrnl > o2.owner >= o2.bound
-  requires m.m.Keys >= o2.AMFO  > o2.AMFX  >= o2.AMFB
-  requires o2 in m.m.Keys
-  requires o2.Ready()
-
-  requires (  o1 == o2   )
-  ensures  (  m.m[o1] == m.m[o2]   )
-{}
-
-
-lemma {:isolate_assertions} fked2(o1 : Object, o2 : Object, m : Klon)
-  requires m.o_amfo <= m.m.Keys   //IN-KLON
-  requires o1 in m.m.Keys
-  requires o2 in m.m.Keys
-  requires acrm: allcertainratio(m)
-  requires allcertainratio(m)
-
-  requires forall o <- m.m.Keys :: o.Ready()
-//   ensures  m.m.Keys >= o1.ntrnl > o1.owner >= o1.bound
-//   ensures  m.m.Keys >= o1.AMFO  > o1.AMFX  >= o1.AMFB
-//   ensures  o1 in m.m.Keys
-//   ensures  o1.Ready()
-//
-//   ensures  m.m.Keys >= o2.ntrnl > o2.owner >= o2.bound
-//   ensures  m.m.Keys >= o2.AMFO  > o2.AMFX  >= o2.AMFB
-//   ensures  o2 in m.m.Keys
-//  ensures  o2.Ready()
-
- requires
-   reveal allcertainratio(), acertainratio(), o2.Ready();
-   forall k <- m.m.Keys :: tragicallyhip(k, m)
-
-//  requires (inside(o1,o2))
-//  ensures  (inside(m.m[o1],m.m[o2]))
-
-//  requires (refDI(o1,o2))
-//  ensures  (refDI(m.m[o1],m.m[o2]))
-
-//  requires (refBI(o1,o2))
-//  ensures  (refBI(m.m[o1],m.m[o2]))
-
- requires (refOK(o1,o2))
- ensures  (refOK(m.m[o1],m.m[o2]))
-{
-  assert allcertainratio(m) by { reveal acrm;}
-  assert o2 in m.m.Keys;
-  assert acertainratio(o2,m) by { reveal acrm, allcertainratio(); }
-  assert
-    var o := o2;
-      && (m.o_amfo <= m.m.Keys)   //IN-KLON
-      && (m.m.Keys >= o.ntrnl > o.owner >= o.bound)
-      && (m.m.Keys >= o.AMFO  > o.AMFX  >= o.AMFB)
-      && (o in m.m.Keys)
-      by { reveal acrm, allcertainratio(), acertainratio(); }
-   assert o2 in m.m.Keys && o2.Ready() by { reveal acrm, allcertainratio(), acertainratio(), o2.Ready(); }
-
-  assert  (refOK(m.m[o1],m.m[o2]));
-}
-
-
-
-lemma fuckenHell(k : Object, v : Object, of : Object, ot : Object, cf : Object, ct: Object, m : Klon)
-{}
-
-predicate dante(o : Object, m : Klon)
-{
-  && o.Ready()
-  && (o in m.m.Keys)
-  && (o.AMFO <= m.m.Keys)
-  && (o.bound <= m.m.Keys)
-  && (o.owner <= m.m.Keys)
-  && (o.ntrnl <= m.m.Keys)
-}
-
-lemma {:isolate_assertions}  fuckenHell2(a : Object, b : Object, c : Object, d : Object, aa : Owner, bb : Owner, cc : Owner, dd : Owner, m : Klon)
-  requires dante(a,m)
-  requires dante(b,m)
-  requires dante(c,m)
-  requires dante(d,m)
-
-  requires m.o_amfo <= m.m.Keys
-  requires aa == tragic3(a, m)
-  requires bb == tragic3(b, m)
-  requires cc == aa - bb
-  requires dd == mapThruKlon(a.AMFO - b.AMFO, m)
-
-  ensures  cc <= dd
-{}
-
-
-lemma {:isolate_assertions} fuckenHell3(a : Object, b : Object, c : Object, d : Object, m : Klon)
-  requires dante(a,m)
-  requires dante(b,m)
-  requires dante(c,m)
-  requires dante(d,m)
-
-  requires m.o_amfo <= m.m.Keys
-  requires forall o <- m.m.Keys ::
-      && (o.AMFO <= m.m.Keys)
-      && (o.bound <= m.m.Keys)
-      && (o.owner <= m.m.Keys)
-      && (o.ntrnl <= m.m.Keys)
-
-  requires allmagic3(m)
-//
-//   requires b != c
-//   requires b != d
-//   requires c != d
-
-  requires c == m.m[a]
-  requires d == m.m[b]
-
-//WORKS..  (isn'r thjis enough)
-// requires inside(b,a)
-// ensures  inside(d,c)
-
-//also fuckenj works
-// requires a == b  // inside(b,a)
-// ensures  c == d  // inside(d,c)
-
-//DOSNT FUCKEN WORK... WHY???
-// requires refOK(a,b) // a == b  // inside(b,a)
-// ensures  refOK(c,d) // c == d  // inside(d,c)
-
-// //WORKS!!!
-// requires refDI(a,b)
-// ensures  refDI(c,d)
-//
-// DOENST FUCKWN WORKS, FUCKER!!
-// requires refBI(a,b)
-// ensures  refBI(c,d)
-
-//SHOULD WORK NOWWW... WHY???
-//requires refOK(a,b) // a == b  // inside(b,a)
-// ensures  refOK(c,d) // c == d  // inside(d,c)
-{
-  // if (  a == b  ) { assert   a == b  ; assert refOK(c,d); return;}
-  // if (refDI(a,b)) { assert refDI(c,d); assert refOK(c,d); return;}
-  // if (refBI(a,b)) { assert refBI(c,d); assert refOK(c,d); return;}
-
-}
-//
-//
-// predicate magic3old(k : Object, v : Object, m : Klon) : ( rv : bool )
-//
-//   requires k !in m.m.Keys
-//   requires v !in m.m.Values
-//
-//   //  requires (forall x <- m.m.Keys :: (not(x.AMFO >= m.o_amfo) <==> (m.m[x] == x)))
-//
-// //  requires (k != v) ==> (v.AMFO >= m.c_amfx)
-// {
-//   //  && (if (k.AMFO >= m.o_amfo)
-//   //       then ((v != k) && (v.AMFO >= m.c_amfx))
-//   //       else ((v == k)))
-//   //  && ((k.AMFX == m.o_amfo) ==> (v.AMFX == m.c_amfx))
-//
-//    && ((k !in m.m.Keys) && (v !in m.m.Values))
-//
-//    && (var satam := subklonKV(m, k, v);
-//     forall i <- m.m.Keys, j <- m.m.Keys :: oxy_NO_builtin(i,j,satam.m[i],satam.m[j],satam))
-// }
-
-predicate magic2(k : Object, v : Object, m : Klon) : ( rv : bool )
-
-  //  requires (forall x <- m.m.Keys :: (not(x.AMFO >= m.o_amfo) <==> (m.m[x] == x)))
-
-//  requires (k != v) ==> (v.AMFO >= m.c_amfx)
-{
-   && (if (k.AMFO >= m.o_amfo)
-        then ((v != k) && (v.AMFO >= m.c_amfx))
-        else ((v == k)))
-   && ((k.AMFX == m.o_amfo) ==> (v.AMFX == m.c_amfx))
-}
-
-lemma allmagic2restored(m' : Klon, k : Object, v : Object, m : Klon)
-  requires k !in m'.m.Keys
-  requires v !in m'.m.Values
-  requires allmagic2(m')
-  requires magic2(k,v,m')
-  requires m == subklonKV(m',k,v)
-  ensures  allmagic2(m)
-{
-  assert v == m.m[k];
-  assert forall mm <- m'.m.Keys :: m'.m[mm]  == m.m[mm];
-  assert forall mm <- m.m.Keys :: ((mm in m'.m.Keys) ==> (m'.m[mm] == m.m[mm]));
-  assert m.m.Keys == m'.m.Keys + {k};
-
-   assert allmagic2(m');
-   assert forall mm <- m'.m.Keys       :: magic2(mm, m.m[mm], m);
-   assert magic2(k,v,m);
-   assert forall mm <- {k}             :: magic2(mm, m.m[mm], m);
-   assert forall mm <- m'.m.Keys + {k} :: magic2(mm, m.m[mm], m);
-   assert forall mm <- m.m.Keys        :: magic2(mm, m.m[mm], m);
-   assert allmagic2(m);
-}
-
-
-predicate magic(k : Object, v : Object, m : Klon) : ( rv : bool )
-
-//  requires (forall x <- m.m.Keys :: (not(x.AMFO >= m.o_amfo) <==> (m.m[x] == x)))
-
-//  requires (k != v) ==> (v.AMFO >= m.c_amfx)
-{
-      (if (k.AMFO >= m.o_amfo)
-        then ((v != k) && (v.AMFO >= m.c_amfx))
-        else ((v == k)))
-}
-
-
-predicate allmagic2(m : Klon)
-{
-  forall x <- m.m.Keys :: magic2(x,m.m[x],m)
-}
-
-predicate allmagic(m : Klon)
-{
-  forall x <- m.m.Keys :: magic(x,m.m[x],m)
-}
-
-lemma wexford3allmagic(m : Klon)
-  ensures allmagic(m) == wexford3(m)
-{}
-
-
-predicate cexford4(m : Klon)
-{
-  && (forall i <- m.m.Keys, j <- m.m.Keys :: cexy_NO_builtin(i,j,m.m[i],m.m[j],m))
-}
-
-
-predicate dexford4(m : Klon)
-{
-  && (forall i <- m.m.Keys, j <- m.m.Keys :: dexy_NO_builtin(i,j,m.m[i],m.m[j],m))
-}
-
-predicate wexford4(m : Klon)
-  requires allmagic2(m)
-{
-  && (forall i <- m.m.Keys, j <- m.m.Keys :: wexy_NO_builtin(i,j,m.m[i],m.m[j],m))
-}
-
-lemma four4(m : Klon)
-  requires allmagic2(m)
-  ensures  cexford4(m) == dexford4(m) == wexford4(m)
-{}
-
-
-predicate wexford3(m : Klon)
-{
-  // && (m.m.Keys   <= m.c)
-  // && (m.m.Values <= m.c)
-
-
-  && (forall x <- m.m.Keys ::
-      (if (x.AMFO >= m.o_amfo)
-        then ((m.m[x] != x) && (m.m[x].AMFO >= m.c_amfx))
-        else ((m.m[x] == x))))
-
-  // && (forall x <- m.m.Keys :: (not(x.AMFO >= m.o_amfo) <==> (m.m[x] == x)))
-
-// && (forall x <- m.m.Keys :: (not(x.AMFO >= m.o_amfo) ==> (m.m[x] == x)))
-
-//  && (forall i <- m.m.Keys, j <- m.m.Keys :: wexy(i,j,m.m[i],m.m[j],m))
-
-}
-
-
-predicate wexford2(m : Klon)
-// note this is built into the SuperKlon
-{
-  // && (m.m.Keys   <= m.c)
-  // && (m.m.Values <= m.c)
-  && (forall x <- m.m.Keys :: (not(x.AMFO >= m.o_amfo) ==> (m.m[x] == x)))
-  && (forall i <- m.m.Keys, j <- m.m.Keys :: refOK(i,j) ==> refOK(m.m[i],m.m[j]))
-}
-
-
-predicate wexford(m : Klon)
-{ forall i <- m.m.Keys, j <- m.m.Keys :: refOK(i,j) ==> refOK(m.m[i],m.m[j]) }
-
-predicate waterford(m : Klon)
-{ forall i <- m.m.Keys, j <- m.m.Keys |  refOK(i,j) ::  refOK(m.m[i],m.m[j]) }
-
-lemma wexwater(m : Klon)
-  ensures wexford(m) == waterford(m)
-{}
-
-
-//[[[[[[[[[[[[[[[[[[[[[[[[[[[[[[[[[[[[[[[[]]]]]]]]]]]]]]]]]]]]]]]]]]]]]]]]]]]]]]]]
-//[[[[[[[[[[[[[[[[[[[[[[[[[[[[[[[[[[[[[[[[]]]]]]]]]]]]]]]]]]]]]]]]]]]]]]]]]]]]]]]]
-
-
-
-
-
-//
-// function AllMyConcievableOwners(a : Object) : Owner
-//   decreases a.AMFO
-//   requires a.Ready()
-//   {
-//     assert a.Ready();
-//     assert forall o <- a.owner ::
-//       && a.AMFO > o.AMFO
-//       && o.Ready();
-//     assert forall oo <- a.owner :: oo.AMFO < a.AMFO;
-//     assert forall oo <- a.owner :: oo.Ready();
-//     set oo <- a.AMFX, ooo <- AllMyConcievableOwners(oo) :: ooo
-//   }
-
-
-
-lemma ASetLessThan(a : Object, aa : set<Object>,  bb : set<Object>, cc : set<Object>)
- requires aa != bb
- requires bb != cc
- requires aa != cc
-
- requires a !in cc
-
-requires aa == bb + {a}
-requires aa >= cc
-
-ensures bb >= cc
- {}
